Work in progress on a computational prover

Theory/Metacategory/ArrowsOnly.v
@@ -248,8 +248,11 @@ Defined.
 
 Ltac destruct_maps :=
   repeat match goal with
+  | [ H : M.find (?X, ?Y) (M.empty _) = Some ?F |- _ ] =>
+    inversion H
   | [ H : M.find (?X, ?Y) (M.add _ _ _) = Some ?F |- _ ] =>
-    apply find_inv in H; destruct H as [[? [? ?]]|]
+    apply find_inv in H;
+    (destruct H as [[? [? ?]]|]; [subst; try nomega|])
   | [ |- ∃ v, M.find _ _ = Some v ] =>
     vm_compute; eexists; reflexivity
 
@@ -301,20 +304,763 @@ Proof.
   apply X0.
 Defined.
 
-Program Definition Two : Metacategory := {|
+(*
+Ltac reflect_on_maps :=
+  try split; intros; simpl in *; destruct_maps; subst;
+  first [ nomega
+        | repeat eexists; clear;
+          first [ instantiate (1 := 0%N); vm_compute; reflexivity
+                | instantiate (1 := 1%N); vm_compute; reflexivity
+                | instantiate (1 := 2%N); vm_compute; reflexivity
+                | instantiate (1 := 3%N); vm_compute; reflexivity
+                | instantiate (1 := 4%N); vm_compute; reflexivity
+                | instantiate (1 := 5%N); vm_compute; reflexivity] ].
+*)
+
+(* Local Obligation Tactic := reflect_on_maps. *)
+
+Inductive term :=
+  | Var : positive -> term
+  | Value : N -> term.
+
+Definition term_beq (x y : term) : bool :=
+  match x, y with
+  | Var x, Var y => (x =? y)%positive
+  | Value x, Value y => (x =? y)%N
+  | _, _ => false
+  end.
+
+Lemma term_beq_sound x y : term_beq x y = true -> x = y.
+Proof.
+  induction x, y; simpl; intros; intuition.
+  - apply Pos.eqb_eq in H; subst; reflexivity.
+  - apply N.eqb_eq in H; subst; reflexivity.
+Defined.
+
+Program Definition term_eq_dec (x y : term) : {x = y} + {x ≠ y} :=
+  match x, y with
+  | Var x,   Var y   => if Pos.eq_dec x y then left _ else right _
+  | Value x, Value y => if N.eq_dec   x y then left _ else right _
+  | _, _ => right _
+  end.
+Next Obligation. congruence. Defined.
+Next Obligation. congruence. Defined.
+Next Obligation. congruence. Defined.
+Next Obligation. congruence. Defined.
+Next Obligation.
+  destruct H.
+  destruct x, y, wildcard', wildcard'0; try discriminate.
+    specialize (H0 p1 p2).
+    intuition.
+  specialize (H n1 n2).
+  intuition.
+Defined.
+Next Obligation.
+  split; intros;
+  unfold not; intros;
+  destruct H1;
+  discriminate.
+Defined.
+Next Obligation.
+  split; intros;
+  unfold not; intros;
+  destruct H1;
+  discriminate.
+Defined.
+
+Section denotation.
+
+Definition subst_term (p : positive) (n : term) (t : term) : term :=
+  match t with
+  | Var x   => if (x =? p)%positive then n else t
+  | Value _ => t
+  end.
+
+Fixpoint subst_term_all (xs : list (positive * term)) t : term :=
+  match xs with
+  | nil => t
+  | cons (p, n) xs => subst_term p n (subst_term_all xs t)
+  end.
+
+Definition term_denote (vars : positive -> N) (x : term) : N :=
+  match x with
+  | Var n => vars n
+  | Value n => n
+  end.
+
+Inductive map_expr : Set :=
+  | Empty : map_expr
+  | Add   : term -> term -> term -> map_expr -> map_expr.
+
+Fixpoint subst_map_expr (p : positive) (n : term) (t : map_expr) : map_expr :=
+  match t with
+  | Empty => Empty
+  | Add x y f m => Add (subst_term p n x) (subst_term p n y)
+                       (subst_term p n f) (subst_map_expr p n m)
+  end.
+
+Fixpoint subst_map_expr_all (xs : list (positive * term)) t : map_expr :=
+  match xs with
+  | nil => t
+  | cons (p, n) xs => subst_map_expr p n (subst_map_expr_all xs t)
+  end.
+
+Fixpoint map_expr_denote (vars : positive -> N) (m : map_expr) : M.t N :=
+  match m with
+  | Empty => M.empty N
+  | Add x y f m' => M.add (term_denote vars x, term_denote vars y)
+                          (term_denote vars f) (map_expr_denote vars m')
+  end.
+
+Inductive formula :=
+  | Maps    : term -> term -> term -> map_expr -> formula
+  | MapsAny : term -> term -> map_expr -> formula
+  | Impl    : formula -> formula -> formula.
+
+Fixpoint subst_formula (p : positive) (n : term) (t : formula) : formula :=
+  match t with
+  | Maps x y f m => Maps (subst_term p n x) (subst_term p n y)
+                         (subst_term p n f) (subst_map_expr p n m)
+  | MapsAny x y m => MapsAny (subst_term p n x) (subst_term p n y)
+                             (subst_map_expr p n m)
+  | Impl a b => Impl a (subst_formula p n b)
+  end.
+
+Fixpoint subst_formula_all (xs : list (positive * term)) t : formula :=
+  match xs with
+  | nil => t
+  | cons (p, n) xs => subst_formula p n (subst_formula_all xs t)
+  end.
+
+Fixpoint formula_denote (vars : positive -> N) (t : formula) : Prop :=
+  match t with
+  | Maps x y f m =>
+    M.MapsTo (term_denote vars x, term_denote vars y) (term_denote vars f)
+             (map_expr_denote vars m)
+  | MapsAny x y m =>
+    M.In (term_denote vars x, term_denote vars y) (map_expr_denote vars m)
+  | Impl p q => formula_denote vars p -> formula_denote vars q
+  end.
+
+Inductive subterm : formula -> formula -> Prop :=
+  | Impl1 : forall t1 t2, subterm t1 (Impl t1 t2)
+  | Impl2 : forall t1 t2, subterm t2 (Impl t1 t2).
+
+Lemma subterm_wf : well_founded subterm.
+Proof.
+  constructor; intros.
+  inversion H; subst; simpl in *;
+  induction y;
+  induction t1 || induction t2;
+  simpl in *;
+  constructor; intros;
+  inversion H0; subst; clear H0;
+  try (apply IHy1; constructor);
+  try (apply IHy2; constructor).
+Defined.
+
+Section partial.
+  Variable P : Prop.
+
+  Inductive partial : Set :=
+  | Proved : P -> partial
+  | Uncertain : partial.
+End partial.
+
+Notation "[ P ]" := (partial P) : type_scope.
+
+Notation "'Yes'" := (Proved _ _) : partial_scope.
+Notation "'No'" := (Uncertain _) : partial_scope.
+
+Local Open Scope partial_scope.
+Delimit Scope partial_scope with partial.
+
+Notation "'Reduce' v" := (if v then Yes else No) (at level 100) : partial_scope.
+Notation "'Reduce' [ T ] v" := (if v then Proved T _ else Uncertain T)
+  (at level 100) : partial_scope.
+Notation "x || y" := (if x then Yes else Reduce y) : partial_scope.
+Notation "x ||[ T ] y" := (if x then Proved T _ else Reduce[T] y) (at level 100) : partial_scope.
+Notation "x && y" := (if x then Reduce y else No) : partial_scope.
+Notation "x &&[ T ] y" := (if x then Reduce[T] y else Uncertain T) (at level 100) : partial_scope.
+
+Local Open Scope lazy_bool_scope.
+
+Fixpoint map_contains (x y : term) (m : map_expr) : option term :=
+  match m with
+  | Empty => None
+  | Add x' y' f' m' =>
+    match term_eq_dec x x' with
+    | left _ =>
+      match term_eq_dec y y' with
+      | left _  => Some f'
+      | right _ => map_contains x y m'
+      end
+    | right _ => map_contains x y m'
+    end
+  end.
+
+Local Obligation Tactic := program_simpl.
+
+Lemma no_subst_term vars p x t :
+  term_denote vars x = vars p
+    -> term_denote vars (subst_term p x t) = term_denote vars t.
+Proof.
+  generalize dependent p.
+  induction t; simpl; intros; auto.
+  - destruct (Pos.eq_dec p p0); subst.
+      rewrite Pos.eqb_refl; auto.
+    apply Pos.eqb_neq in n; rewrite n; auto.
+Qed.
+
+Lemma no_subst_map_expr vars p x t :
+  term_denote vars x = vars p
+    -> map_expr_denote vars (subst_map_expr p x t) = map_expr_denote vars t.
+Proof.
+  generalize dependent p.
+  induction t; simpl; intros; auto.
+  - rewrite IHt, !no_subst_term; auto.
+Qed.
+
+Lemma no_subst_formula vars p x t :
+  term_denote vars x = vars p
+    -> formula_denote vars (subst_formula p x t) = formula_denote vars t.
+Proof.
+  generalize dependent p.
+  induction t; simpl; intros; auto.
+  - rewrite !no_subst_term, !no_subst_map_expr; auto.
+  - rewrite !no_subst_term, !no_subst_map_expr; auto.
+  -intuition.
+   rewrite IHt2; auto.
+Qed.
+
+Lemma subst_map_expr_all_Empty defs :
+  subst_map_expr_all defs Empty = Empty.
+Proof.
+  induction defs; simpl; auto.
+  destruct a.
+  rewrite IHdefs; reflexivity.
+Qed.
+
+Lemma subst_map_expr_all_Add defs x y f m :
+  subst_map_expr_all defs (Add x y f m) =
+  Add (subst_term_all defs x) (subst_term_all defs y)
+      (subst_term_all defs f) (subst_map_expr_all defs m).
+Proof.
+  induction defs; simpl; auto.
+  destruct a.
+  rewrite IHdefs; reflexivity.
+Qed.
+
+Lemma subst_formula_all_Maps defs x y f m :
+  subst_formula_all defs (Maps x y f m) =
+  Maps (subst_term_all defs x) (subst_term_all defs y)
+       (subst_term_all defs f) (subst_map_expr_all defs m).
+Proof.
+  induction defs; simpl; auto.
+  destruct a.
+  rewrite IHdefs; reflexivity.
+Qed.
+
+Lemma subst_formula_all_MapsAny defs x y m :
+  subst_formula_all defs (MapsAny x y m) =
+  MapsAny (subst_term_all defs x) (subst_term_all defs y)
+          (subst_map_expr_all defs m).
+Proof.
+  induction defs; simpl; auto.
+  destruct a.
+  rewrite IHdefs; reflexivity.
+Qed.
+
+Lemma subst_formula_all_Impl defs p q :
+  subst_formula_all defs (Impl p q) = Impl p (subst_formula_all defs q).
+Proof.
+  induction defs; simpl; auto.
+  destruct a.
+  rewrite IHdefs; reflexivity.
+Defined.
+
+Definition check_def (defs : list (positive * term)) (t v : term) : bool :=
+  match t with
+  | Var t =>
+    let fix check xs v v' :=
+        match xs return bool with
+        | nil => true
+        | cons (x, x') xs =>
+          match Pos.eq_dec v x with
+          | left _ =>
+            match term_eq_dec v' x' with
+            | left _  => true
+            | right _ => false
+            end
+          | right _ => check xs v v'
+          end
+        end in
+    check defs t v
+  | _ => true
+  end.
+
+(* The only job of formula_forward at the moment is to accumulate variable
+   definitions. *)
+Program Definition formula_forward (t : formula)
+        (vars : positive -> N) (defs : list (positive * term))
+        (hyp : formula)
+        (cont : ∀ vars' defs', [formula_denote vars' (subst_formula_all defs' t)]) :
+  [formula_denote vars hyp -> formula_denote vars (subst_formula_all defs t)] :=
+  let mk v v' xs :=
+      match v return list (positive * term) with
+      | Var v => cons (v, v') xs
+      | _ => xs
+      end in
+  match hyp with
+  | Maps x y f m =>
+    let fix go n : [formula_denote vars (Maps x y f n)
+                      -> formula_denote vars (subst_formula_all defs t)] :=
+        match n with
+        | Empty => Yes
+        | Add x' y' f' m' =>
+          match check_def defs x x' with | true =>
+          match check_def defs y y' with | true =>
+          match check_def defs f f' with | true =>
+            cont vars (mk x x' (mk y y' (mk f f' defs))) && go m'
+          | false => Reduce (go m') end
+          | false => Reduce (go m') end
+          | false => Reduce (go m') end
+        end in go m
+  | MapsAny x y m =>
+    let fix go n : [formula_denote vars (MapsAny x y n)
+                      -> formula_denote vars (subst_formula_all defs t)] :=
+        match n with
+        | Empty => Yes
+        | Add x' y' f' m' =>
+          match check_def defs x x' with | true =>
+          match check_def defs y y' with | true =>
+            cont vars (mk x x' (mk y y' defs)) && go m'
+          | false => Reduce (go m') end
+          | false => Reduce (go m') end
+        end in go m
+  | Impl _ _ => Reduce (cont vars defs)
+  end.
+Next Obligation.
+  simplify_maps.
+  clear go cont.
+  destruct H2.
+  simpl in *.
+  destruct x, y, f; simpl in *;
+  repeat (rewrite no_subst_formula in H; auto); auto.
+Defined.
+Next Obligation.
+  simplify_maps.
+  clear go cont.
+  destruct H1.
+  simpl in *.
+  destruct x, y, f; simpl in *;
+  repeat (rewrite no_subst_formula in H; auto); auto.
+Admitted.
+Next Obligation.
+  simplify_maps.
+  clear go cont.
+  destruct H1.
+  simpl in *.
+  destruct x, y, f; simpl in *;
+  repeat (rewrite no_subst_formula in H; auto); auto.
+Admitted.
+Next Obligation.
+  simplify_maps.
+  clear go cont.
+  destruct H1.
+  simpl in *.
+  destruct x, y, f; simpl in *;
+  repeat (rewrite no_subst_formula in H; auto); auto.
+Admitted.
+Next Obligation.
+  apply F.empty_in_iff in H.
+  contradiction.
+Defined.
+Next Obligation.
+  simpl in H1.
+  apply F.add_in_iff in H1.
+  destruct H1; auto.
+  clear H0 go cont.
+  destruct H1.
+  simpl in *.
+  destruct x, y; simpl in *;
+  repeat (rewrite no_subst_formula in H; auto); auto.
+Defined.
+Next Obligation.
+  apply F.add_in_iff in H0.
+  destruct H0; auto.
+  clear H go cont.
+  destruct H0.
+  simpl in *.
+Admitted.
+Next Obligation.
+  apply F.add_in_iff in H0.
+  destruct H0; auto.
+  clear H go cont.
+  destruct H0.
+  simpl in *.
+Admitted.
+
+Lemma map_contains_MapsTo vars x y f m :
+  Some f = map_contains x y m ->
+  M.MapsTo (term_denote vars x, term_denote vars y)
+           (term_denote vars f) (map_expr_denote vars m).
+Proof.
+  intros.
+  apply F.find_mapsto_iff.
+  induction m; simpl; intros.
+    discriminate.
+  simpl in *.
+  destruct (term_eq_dec x t); subst.
+    destruct (term_eq_dec y t0); subst.
+      inversion H; subst.
+      simplify_maps.
+    rewrite F.add_neq_o; auto; simpl.
+    admit.
+  rewrite F.add_neq_o; auto; simpl.
+  admit.
+Admitted.
+
+Lemma subst_formula_all_Impl_impl {defs p q t} :
+  Impl p q = subst_formula_all defs t ->
+    ∃ q', Impl p q' = t ∧ q = subst_formula_all defs q'.
+Proof.
+  intros.
+  induction t.
+  - induction defs; simpl in *.
+      discriminate.
+    destruct a.
+    rewrite subst_formula_all_Maps in H; simpl in H.
+    discriminate.
+  - induction defs; simpl in *.
+      discriminate.
+    destruct a.
+    rewrite subst_formula_all_MapsAny in H; simpl in H.
+    discriminate.
+  - rewrite subst_formula_all_Impl in H; simpl in H.
+    inversion H; subst.
+    eexists.
+    split; reflexivity.
+Qed.
+
+Lemma formula_denote_Impl_forward {vars defs p q} :
+  [formula_denote vars p → formula_denote vars (subst_formula_all defs q)]
+    -> [formula_denote vars (Impl p q)].
+Proof.
+  intros.
+  simpl in *.
+Abort.
+
+Lemma subterm_subst_formula_all defs p x :
+  subterm x (Impl p x) ->
+  subterm (subst_formula_all defs x) (Impl p x).
+Proof.
+Abort.
+
+Program Fixpoint formula_backward (t : formula)
+        (vars : positive -> N) (defs : list (positive * term))
+        {wf subterm t} : [formula_denote vars (subst_formula_all defs t)] :=
+  match t with
+  | Maps x y f m =>
+    match map_contains (subst_term_all defs x) (subst_term_all defs y)
+                       (subst_map_expr_all defs m) with
+    | Some f' => Reduce (term_eq_dec f' (subst_term_all defs f))
+    | None => No
+    end
+  | MapsAny x y m =>
+    match map_contains (subst_term_all defs x) (subst_term_all defs y)
+                       (subst_map_expr_all defs m) with
+    | Some _ => Yes
+    | None => No
+    end
+  | Impl p q =>
+    _ (formula_forward q vars defs p
+                       (fun vars' defs' => formula_backward q vars' defs'))
+  end.
+Next Obligation.
+  rewrite subst_formula_all_Maps; simpl.
+  apply map_contains_MapsTo; auto.
+Defined.
+Next Obligation.
+  rewrite subst_formula_all_MapsAny; simpl.
+  apply in_mapsto_iff.
+  eexists.
+  apply map_contains_MapsTo; auto.
+  apply Heq_anonymous.
+Defined.
+Next Obligation.
+  rewrite subst_formula_all_Impl; auto.
+Defined.
+Next Obligation.
+  destruct q; constructor.
+Defined.
+Next Obligation. apply measure_wf, subterm_wf. Defined.
+
+Goal
+  if formula_backward
+       (Impl (Maps (Var 1%positive) (Var 2%positive) (Var 3%positive)
+                   (Add (Value 1%N) (Value 1%N) (Value 1%N) Empty))
+             (Maps (Var 1%positive) (Var 2%positive) (Var 3%positive)
+                   (Add (Value 1%N) (Value 1%N) (Value 1%N) Empty)))
+       (fun v => 9%N) nil then True else False.
+Proof.
+  vm_compute.
+  constructor.
+Qed.
+
+Definition formula_tauto : forall (vars : positive -> N) (t : formula),
+  [formula_denote vars t].
+Proof.
+  intros; refine (Reduce (formula_backward t vars nil)); auto.
+Defined.
+
+Require Import Coq.quote.Quote.
+
+Definition partialOut (P : Prop) (x : [P]) :=
+  match x return (match x with
+                  | Proved _ _ => P
+                  | Uncertain _ => True
+                  end) with
+  | Proved _ pf => pf
+  | Uncertain _ => I
+  end.
+
+Ltac inList x xs :=
+  match xs with
+  | tt => false
+  | (x, _) => true
+  | (_, ?xs') => inList x xs'
+  end.
+
+Ltac addToList x xs :=
+  let b := inList x xs in
+  match b with
+  | true => xs
+  | false => constr:((x, xs))
+  end.
+
+Ltac lookup x xs :=
+  match xs with
+  | (x, _) => constr:(1%positive)
+  | (_, ?xs') =>
+    let n := lookup x xs' in
+    constr:(Pos.succ n)
+  end.
+
+Ltac functionalize xs :=
+  let rec loop n xs' :=
+    lazymatch xs' with
+    | (?x, tt) => constr:(fun _ : positive => x)
+    | (?x, ?xs'') =>
+      let f := loop (Pos.succ n) xs'' in
+      constr:(fun m : positive => if (m =? n)%positive then x else f m)
+    end in
+  loop (1%positive) xs.
+
+Ltac allVar xs e :=
+  match e with
+  | N0 => xs
+  | Npos _ => xs
+  | ?x => addToList x xs
+  end.
+
+Ltac allVars xs e :=
+  match e with
+  | M.MapsTo (?X, ?Y) ?F _ =>
+    let xs := allVar xs X in
+    let xs := allVar xs Y in
+    allVar xs F
+  | M.In (?X, ?Y) _ =>
+    let xs := allVar xs X in
+    allVar xs Y
+  | ?P -> ?Q =>
+    let xs := allVars xs P in
+    allVars xs Q
+  | _ => xs
+  end.
+
+Ltac reifyValue env t :=
+  match t with
+  | N0 => constr:(Value N0)
+  | Npos ?X =>
+    constr:(Value (Npos X))
+  | ?X =>
+    let v := lookup X env in
+    constr:(Var v)
+  end.
+
+Ltac reifyMapTerm env t :=
+  match t with
+  | M.empty _ => constr:(Empty)
+  | M.add (?X, ?Y) ?F ?M =>
+    let x := reifyValue env X in
+    let y := reifyValue env Y in
+    let f := reifyValue env F in
+    let m := reifyMapTerm env M in
+    constr:(Add x y f m)
+  end.
+
+Ltac reifyTerm env t :=
+  match t with
+  | M.MapsTo (?X, ?Y) ?F ?M =>
+    let x := reifyValue env X in
+    let y := reifyValue env Y in
+    let f := reifyValue env F in
+    let m := reifyMapTerm env M in
+    constr:(Maps x y f m)
+  | M.In (?X, ?Y) ?M =>
+    let x := reifyValue env X in
+    let y := reifyValue env Y in
+    let m := reifyMapTerm env M in
+    constr:(MapsAny x y m)
+  | ?P -> ?Q =>
+    let p := reifyTerm env P in
+    let q := reifyTerm env Q in
+    constr:(Impl p q)
+  end.
+
+Ltac reify' :=
+  match goal with
+  | [ |- ?X ] =>
+    let xs  := allVars tt X in
+    let env := functionalize xs in
+    let r1  := reifyTerm xs X in
+    pose xs;
+    pose env;
+    pose r1
+  end.
+
+Ltac reify :=
+  match goal with
+  | [ |- ?X ] =>
+    let xs  := allVars tt X in
+    let env := functionalize xs in
+    let r1  := reifyTerm xs X in
+    pose xs;
+    pose env;
+    pose r1;
+    change (formula_denote env r1)
+  end.
+
+Lemma formula_sound vars t :
+  (if formula_tauto vars t then True else False) -> formula_denote vars t.
+Proof.
+  unfold formula_tauto.
+  destruct t; simpl; intros.
+  - induction m; simpl in *.
+      contradiction.
+    destruct (formula_backward (Maps _ _ _ (Add _ _ _ m)) vars []) eqn:?; auto.
+    contradiction.
+  - induction m; simpl in *.
+      contradiction.
+    destruct (formula_backward (MapsAny _ _ (Add _ _ _ m)) vars []) eqn:?; auto.
+    contradiction.
+  - destruct (formula_backward (Impl _ _) vars []) eqn:?; auto.
+    contradiction.
+Qed.
+
+Ltac solve_map := reify; apply formula_sound; vm_compute; auto.
+
+Example map_decide_test  x y f :
+  M.MapsTo (elt:=N) (x, y) f (M.add (0%N, 0%N) 0%N (M.add (1%N, 1%N) 1%N (M.empty _))) ->
+  M.MapsTo (elt:=N) (x, y) f (M.add (0%N, 0%N) 0%N (M.add (1%N, 1%N) 1%N (M.empty _))).
+Proof. solve_map. Qed.
+
+Time Program Definition Zero : Metacategory := {|
+  pairs := [map]
+|}.
+
+Ltac prepare_maps :=
+  repeat lazymatch goal with
+  | [ |- ∃ v, M.find _ _ = Some v ] =>
+    apply find_mapsto_iff_ex, in_mapsto_iffT
+  | [ |- M.find _ _ = Some _ ] =>
+    apply F.find_mapsto_iff
+  | [ H : M.find _ (M.empty _) = Some _ |- _ ] => inversion H
+  | [ H : M.find _ _ = Some ?F |- _ ] =>
+    apply F.find_mapsto_iff in H; revert H
+  | [ H : M.MapsTo _ _ (M.empty _) |- _ ] =>
+    contradiction (proj1 (F.empty_mapsto_iff _ _) H)
+  end.
+
+Ltac map_decide := prepare_maps; solve_map.
+
+Local Obligation Tactic :=
+  repeat eexists; simpl; try split; intros;
+  first [ map_decide
+        | instantiate (1:=0%N); map_decide
+        | instantiate (1:=1%N); map_decide
+        | instantiate (1:=2%N); map_decide
+        | instantiate (1:=3%N); map_decide
+        | instantiate (1:=4%N); map_decide
+        | instantiate (1:=5%N); map_decide ].
+
+Time Program Definition One : Metacategory := {|
+  pairs := [map (0, 0) +=> 0 ]%N
+|}.
+
+Local Obligation Tactic := simpl; intros.
+
+Time Program Definition Two : Metacategory := {|
   pairs := [map (0, 0) +=> 0
            ;    (1, 1) +=> 1
-           ;    (1, 2) +=> 2
-           ;    (2, 0) +=> 2 ]%N
+
+           ;    (2, 0) +=> 2
+           ;    (1, 2) +=> 2 ]%N
 |}.
-Next Obligation. destruct_maps; nomega. Defined.
-Next Obligation. split; intros; destruct_maps; subst; nomega. Qed.
 Next Obligation.
-  destruct_maps; subst;
-  eexists; eexists; intros; clear; split;
-  first [ instantiate (1 := 0%N); vm_compute; reflexivity
-        | instantiate (1 := 1%N); vm_compute; reflexivity ].
-Defined.
+  prepare_maps.
+  reify.
+  compute [Pos.succ] in *.
+  apply formula_sound.
+  vm_compute.
+  simpl.
+
+Time Program Definition Three : Metacategory := {|
+  pairs := [map (0, 0) +=> 0
+           ;    (1, 1) +=> 1
+           ;    (2, 2) +=> 2
+
+           ;    (3, 0) +=> 3
+           ;    (1, 3) +=> 3
+
+           ;    (4, 1) +=> 4
+           ;    (2, 4) +=> 4
+
+           ;    (5, 0) +=> 5
+           ;    (2, 5) +=> 5
+           ;    (4, 3) +=> 5 ]%N
+|}.
+
+Time Program Definition Four : Metacategory := {|
+  pairs := [map (0, 0) +=> 0
+           ;    (1, 1) +=> 1
+           ;    (2, 2) +=> 2
+           ;    (3, 3) +=> 3
+
+           ;    (4, 0) +=> 4
+           ;    (1, 4) +=> 4
+
+           ;    (5, 1) +=> 5
+           ;    (2, 5) +=> 5
+
+           ;    (6, 2) +=> 6
+           ;    (3, 6) +=> 6
+
+           ;    (7, 0) +=> 7
+           ;    (2, 7) +=> 7
+
+           ;    (8, 1) +=> 8
+           ;    (3, 8) +=> 8
+
+           ;    (9, 0) +=> 9
+           ;    (3, 9) +=> 9
+
+           ;    (5, 4) +=> 7
+           ;    (6, 5) +=> 8
+           ;    (7, 6) +=> 9
+           ;    (8, 4) +=> 9 ]%N
+|}.
 
 Ltac reflect_on_pairs X Y F D C :=
   repeat (
